proofs 1-3 very simple... dealing w/ subsumption
So, it turns out with the simple typing rules written as they are you
end up needing subsumption *all over the place* — for example, any time
you’re reasoning about bools and an explicit #t or #f appears it’s very
possible you’ll need to use subsumption to make things work, since
although both #t and #f *are* bools, they are not equal to bool (since
#t is of type tTrue, #f is of type tFalse, and bool is (tUnion tTrue
tFalse). This makes building Ltac tactics which automatically solve
these “simple examples” more difficult than would be ideal, since often
applying the “fitting relational constructor” leads you directly down a
path where equality is required =(

Saving now… may look into making all typing judgements resort to
subtype checking instead of the current practice of all being literal
(i.e. using equality) and allowing for subsumption when necessary.
We’ll see…

LambdaTR.v
@@ -1,5 +1,4 @@
 
-
 Require Import LibTactics.
 Require Import List.
 Require Import ListSet.
@@ -242,10 +241,6 @@ Inductive exp : Type :=
 | expCons : exp -> exp -> exp
 | expLet : id -> exp -> exp -> exp.
 
-Notation "(and' x y )" := (expIf x y expF).
-Notation "(or' x y )" := (expIf x expT y).
-
-
 Notation car' := (expPrimop (prim_p op_car)).
 Notation cdr' := (expPrimop (prim_p op_cdr)).
 Notation add1' := (expPrimop (prim_c op_add1)).
@@ -264,19 +259,8 @@ if exp_eqdec x y then true else false.
 
 Inductive SubObj : relation obj :=
 | SO_Refl : forall x, SubObj x x
-| SO_Top : forall x, SubObj x objnil.
+| SO_Top : forall x, SubObj objnil x.
 Hint Constructors SubObj.
-
-Theorem sub_obj : forall x y,
-{SubObj x y} + {~ SubObj x y}.
-Proof.
-  intros x y.
-  destruct (obj_eqdec x y) as [Heq | Hneq].
-  left; crush.
-  destruct y. auto.
-  right; intro contra.
-  inversion contra; crush.
-Defined.
 
 Inductive isUnion : type -> Prop :=
 | isU : forall t1 t2, isUnion (tUnion t1 t2).
@@ -434,11 +418,11 @@ with UpdatedLookupSet : bool -> type -> obj -> lookupset -> lookupset -> Prop :=
 
 with UpdatedLookup : bool -> type -> obj -> typelookup -> typelookup -> Prop :=
 | UL_Some :
-    forall b t t' pth pth' x tl o updated,
+    forall b t t' pth pth' pth'' x tl updated,
+      pth'' = (pth ++ pth') ->
       tl (objπ pth' x) = t' ->
       UpdatedType t' (b, t) pth updated ->
-      o = (objπ (pth ++ pth') x) ->
-      UpdatedLookup b t o (Some tl) (extend_lookup (objπ pth' x) updated (Some tl))
+      UpdatedLookup b t (objπ pth'' x) (Some tl) (extend_lookup (objπ pth' x) updated (Some tl))
 | UL_None :
     forall b t o,
     UpdatedLookup b t o None None
@@ -467,10 +451,10 @@ with Restricted : type -> type -> type -> Prop :=
     forall t σ,
       common_subtype t σ = false ->
       Restricted t σ tBottom
-| RES_Bottom_Left :
+| RES_Bottom_l :
     forall σ,
       Restricted tBottom σ tBottom
-| RES_Bottom_Right :
+| RES_Bottom_r :
     forall σ,
       Restricted σ tBottom tBottom
 | RES_U :
@@ -486,20 +470,17 @@ with Restricted : type -> type -> type -> Prop :=
       Restricted t σ t
 | RES_NonSub :
     forall t σ,
-      common_subtype t σ = true ->      
+      possible_subtype t σ = false -> 
+      common_subtype t σ = true ->
       (~isUnion t) ->
       NonSubtype t σ ->
       Restricted t σ σ
 
 with Removed : type -> type -> type -> Prop :=
-| REM_Bot :
-    forall t σ,
-      Subtype t σ ->
-      Removed t σ tBottom
-| REM_Bottom_Left :
+| REM_Bottom_l :
     forall σ,
       Removed tBottom σ tBottom
-| REM_Bottom_Right :
+| REM_Bottom_r :
     forall t,
       Removed t tBottom t
 | REM_Union :
@@ -507,7 +488,11 @@ with Removed : type -> type -> type -> Prop :=
       Removed t1 σ t1' ->
       Removed t2 σ t2' ->
       Removed (tUnion t1 t2) σ (tUnion t1' t2')
-| REM_nop :
+| REM_Sub :
+    forall t σ,
+      Subtype t σ ->
+      Removed t σ tBottom
+| REM_NonSub :
     forall t σ,
       NonSubtype t σ -> 
       (~isUnion t) ->
@@ -754,8 +739,6 @@ with NonSubtype : type -> type -> Prop :=
       CannotProve fE fE' ->
       NonSubtype (tλ x σ tE fE o t) (tλ x σ' tE' fE' o' t')      
 
-| NST_temp : forall t1 t2, NonSubtype t1 t2
-
 (* Proves: One environment (lhs) has the typing information
    to prove the conclusion in the other environment (the rhs). *)
 with Proves : relation env  :=
@@ -840,14 +823,221 @@ with ProvesTyping : lookupset -> bool -> type -> obj -> Prop :=
 | PT_False_Atom :
     forall b t o,
       ProvesTyping (tls_atom None) b t o.
+
+Ltac tryUE :=
+  first [(eapply UE_Empty) | 
+         (eapply UE_Fact) |
+         (eapply UE_Or) |
+         (eapply UE_False)].
+
+Ltac tryULS :=
+  first [(eapply ULS_Atom) |
+         (eapply ULS_Cons)].
+
+Ltac tryUL :=
+  first [(eapply UL_Some) |
+         (eapply UL_None)].
+
+Ltac tryUT :=
+  first [(eapply UT_T) |
+         (eapply UT_NT) |
+         (eapply UT_Car) |
+         (eapply UT_Cdr) ].
+
+Ltac tryRES :=
+  first [(eapply RES_Bottom_l) |
+         (eapply RES_Bottom_r) |
+         (eapply RES_U) |
+         ((eapply RES_Bottom); compute;
+          match goal with
+          | |- common_subtype ?t ?σ = false => compute; first [reflexivity | fail 1]
+          | |- false = false => compute; reflexivity
+          | |- true = false => fail 1
+          | |- _ => eauto
+          end) |
+         ((eapply RES_NonSub); compute;
+          match goal with
+          | |- possible_subtype ?t ?σ = false => compute; first [reflexivity | fail 1];
+            match goal with
+            | |- common_subtype ?t ?σ = true => compute; first [reflexivity | fail 2]
+            | |- common_subtype ?t ?σ = false => fail 1
+            | |- false = true => fail 1
+            | |- true = false => fail 1
+            | |- _ => eauto
+            end
+          | |- common_subtype ?t ?σ = true => compute; first [reflexivity | fail 1]
+          | |- possible_subtype ?t ?σ = true => fail 1
+          | |- common_subtype ?t ?σ = false => fail 1
+          | |- false = true => fail 1
+          | |- true = false => fail 1
+          | |- _ => eauto
+          end) |
+         (eapply RES_Sub)].
+
+Ltac tryT :=
+  first [(eapply T_Const_isnum) |
+        (eapply T_Const_isproc) |
+        (eapply T_Const_isbool) |
+        (eapply T_Const_iscons) |
+        (eapply T_Const_add1) |
+        (eapply T_Const_iszero) |
+        (eapply T_Num) |
+        (eapply T_True) |
+        (eapply T_False) |
+        (eapply T_Var) |
+        (eapply T_Abs) |
+        (eapply T_App) |
+        (eapply T_If) |
+        (eapply T_Cons) |
+        (eapply T_Car) |
+        (eapply T_Cdr) |
+        (eapply T_Let)].
+(* Removed Subsume since it always works *)  
+
+
+Ltac tryS :=
+  first [(eapply S_Refl) |
+        (eapply S_Top) |
+        (eapply S_UnionSub) |
+        (eapply S_Fun) |
+        (eapply S_Pair) |
+        (match goal with
+         | |- Subtype ?t1 (tUnion ?t1 ?t2) => 
+           eapply S_UnionSuper_l
+         | |- Subtype ?t2 (tUnion ?t1 ?t2) => 
+           eapply S_UnionSuper_r
+         | |- Subtype ?t1 (tUnion (tUnion ?t1 ?t2) ?t3) => 
+           eapply S_UnionSuper_l; eapply S_UnionSuper_l
+         | |- Subtype ?t2 (tUnion (tUnion ?t1 ?t2) ?t3) => 
+           eapply S_UnionSuper_l; eapply S_UnionSuper_r
+         | |- Subtype ?t2 (tUnion ?t1 (tUnion ?t2 ?t3)) => 
+           eapply S_UnionSuper_r; eapply S_UnionSuper_l
+         | |- Subtype ?t3 (tUnion ?t1 (tUnion ?t2 ?t3)) => 
+           eapply S_UnionSuper_r; eapply S_UnionSuper_r
+        end)].
+
+Ltac tryNS :=
+  first [(eapply NS_Trivial) |
+        (eapply NS_UnionSuper) |
+        (eapply NS_UnionSub_l) |
+        (eapply NS_UnionSub_r) |
+        (eapply NS_Abs_arg) |
+        (eapply NS_Abs_result) |
+        (eapply NS_Abs_obj) |
+        (eapply NS_Abs_tEnv) |
+        (eapply NS_Abs_fEnv)].
+
+
+Ltac tryREM :=
+  first [(eapply REM_Bottom_l) |
+         (eapply REM_Bottom_r) |
+         (eapply REM_Union) |
+         (match goal with
+            | |- Removed ?t1 ?t2 ?tr =>
+              assert (Subtype t1 t2) by solve [ tryS; crush ];
+            match goal with
+              | |- Subtype t1 t2 => fail 1
+              | _ => eapply REM_Sub
+            end
+            | |- Removed ?t1 ?t2 ?tr =>
+              assert (NonSubtype t1 t2) by solve [ tryNS; crush ];
+            match goal with
+              | |- NonSubtype t1 t2 => fail 1
+              | _ => eapply REM_NonSub
+            end
+          end)].
+
+
+Ltac tryP :=
+  first [(eapply P_Refl) |
+        (eapply P_False) |
+        (eapply P_Fact_rhs) |
+        (eapply P_Or_rhs_l) |
+        (eapply P_Or_rhs_r) |
+        (eapply P_Or_lhs) |
+        (eapply P_Fact_lhs)].
+
+Ltac tryCP :=
+  first [(eapply CP_Fact) |
+        (eapply CP_Or)].
+
+Ltac tryPT :=
+  first [(eapply PT_Atom) |
+        (eapply PT_FAtom) |
+        (eapply PT_Sub_Cons) |
+        (eapply PT_False_Atom) |
+        (eapply PT_False_Cons) |
+        (eapply PT_FCons_new) |
+        (eapply PT_FCons_prev)].
+
+Lemma then_else_eq : forall (T:Type) (P1 P2:Prop) (test: sumbool P1 P2) (Q:T),
+(if test then Q else Q) = Q.
+Proof.
+  crush.
+Qed.
+Hint Rewrite then_else_eq.
+
+Lemma if_id_eqdec_refl : forall (T:Type) x (t1 t2: T),
+(if id_eqdec x x then t1 else t2) = t1.
+Proof.
+  intros T x t1 t2.
+  destruct (id_eqdec x x); auto. tryfalse.
+Qed.
+Hint Rewrite if_id_eqdec_refl.
+
+Lemma if_obj_eqdec_refl : forall (T:Type) x (t1 t2: T),
+(if obj_eqdec x x then t1 else t2) = t1.
+Proof.
+  intros T x t1 t2.
+  destruct (obj_eqdec x x); auto. tryfalse.
+Qed.
+Hint Rewrite if_obj_eqdec_refl.
+
+Lemma neq_id_neq : forall (T:Type) x y (P Q:T),
+x <> y ->
+((if (id_eqdec x y) then P else Q) = Q).
+Proof.
+  intros.
+  destruct (id_eqdec x y); crush.
+Qed.
+
+Lemma neq_obj_neq : forall (T:Type) x y (P Q:T) pth1 pth2,
+x <> y ->
+((if (obj_eqdec (objπ pth1 x) (objπ pth2 y)) then P else Q) = Q).
+Proof.
+  intros.
+  destruct (obj_eqdec (objπ pth1 x) (objπ pth2 y)); crush.
+Qed.
+
+Lemma if_type_eqdec_refl : forall (T:Type) x (t1 t2: T),
+(if type_eqdec x x then t1 else t2) = t1.
+Proof.
+  intros T x t1 t2.
+  destruct (type_eqdec x x); auto. tryfalse.
+Qed.
+Hint Rewrite if_type_eqdec_refl.
+
+Ltac crushTR :=
+repeat (try (erewrite 
+               then_else_eq 
+               || erewrite if_id_eqdec_refl 
+               || erewrite if_obj_eqdec_refl 
+               || erewrite if_type_eqdec_refl
+               || erewrite neq_obj_neq
+               || erewrite neq_id_neq
+               || tryUE || tryULS || tryUL || tryUT 
+               || tryRES || tryREM 
+               || tryT || tryS || tryNS || tryP || tryCP 
+               || tryPT || eauto || crush)).
+(*
 Hint Constructors UpdatedEnv UpdatedLookupSet UpdatedLookup UpdatedType 
 Restricted Removed Typing Subtype NonSubtype Proves CannotProve.
 Hint Resolve PT_Atom PT_Sub_Cons PT_FAtom PT_FCons_prev PT_FCons_new.
-
+*)
 
 Theorem P_Empty : forall E,
 Proves E envEmpty.
-Proof with crush. 
+Proof with crushTR. 
   intros E.
   induction E...
 Qed.
@@ -899,36 +1089,12 @@ Hint Rewrite app_envEmpty_r.
 Lemma empty_proves_top : forall x E,
 Proves envEmpty E ->
 Proves envEmpty (envFact true tTop (var x) E).
-Proof.
+Proof with crushTR.
   intros x E HE.
-  eapply P_Fact_rhs. auto. eauto. eapply (PT_Atom tTop tTop). auto.
-  auto.
+  eapply P_Fact_rhs...
 Qed.
 Hint Resolve empty_proves_top.
 
-Lemma if_id_eqdec_refl : forall (T:Type) x (t1 t2: T),
-(if id_eqdec x x then t1 else t2) = t1.
-Proof.
-  intros T x t1 t2.
-  destruct (id_eqdec x x); auto. tryfalse.
-Qed.
-Hint Rewrite if_id_eqdec_refl.
-
-Lemma if_obj_eqdec_refl : forall (T:Type) x (t1 t2: T),
-(if obj_eqdec x x then t1 else t2) = t1.
-Proof.
-  intros T x t1 t2.
-  destruct (obj_eqdec x x); auto. tryfalse.
-Qed.
-Hint Rewrite if_obj_eqdec_refl.
-
-Lemma if_type_eqdec_refl : forall (T:Type) x (t1 t2: T),
-(if type_eqdec x x then t1 else t2) = t1.
-Proof.
-  intros T x t1 t2.
-  destruct (type_eqdec x x); auto. tryfalse.
-Qed.
-Hint Rewrite if_type_eqdec_refl.
 
 Lemma top_not_union :
 ~ isUnion tTop.
@@ -953,89 +1119,8 @@ Proof. intros t1 t2 contra; inversion contra. Qed.
 Hint Resolve top_not_union num_not_union true_not_union
 false_not_union λ_not_union pair_not_union.
 
-Lemma then_else_eq : forall (T:Type) (P1 P2:Prop) (test: sumbool P1 P2) (Q:T),
-(if test then Q else Q) = Q.
-Proof.
-  crush.
-Qed.
-Hint Rewrite then_else_eq.
-
-Ltac eautoUE :=
-repeat 
-  (try 
-     (match goal with
-        | |- UpdatedEnv envEmpty ?tl => (eapply UE_Empty)
-        | |- UpdatedEnv (envFalse ?E) ?tl => (eapply UE_False)
-        | |- UpdatedEnv (envFact ?b ?t ?o ?tl) ?E => (eapply UE_Fact)
-        | |- UpdatedEnv (envOr ?E1 ?E2) ?tl => (eapply UE_Or)
-      end)).
-  
-
-Ltac eautoULS :=
-repeat 
-  (try 
-     (match goal with
-        | |- UpdatedLookupSet ?b ?t ?o (tls_atom ?tl) => (eapply ULS_Atom)
-        | |- UpdatedLookupSet ?b ?t ?o (tls_cons ?tl ?tls) => (eapply UE_False)
-      end)).
 
 
-Ltac eautoT :=
-try
-  (repeat 
-     (match goal with
-        | |- Typing ?E isnum' ?t ?tE ?fE ?o => (eapply T_Const_isnum)
-        | |- Typing ?E isproc' ?t ?tE ?fE ?o => (eapply T_Const_isproc)
-        | |- Typing ?E isbool' ?t ?tE ?fE ?o => (eapply T_Const_isbool)
-        | |- Typing ?E iscons' ?t ?tE ?fE ?o => (eapply T_Const_iscons)
-        | |- Typing ?E add1' ?t ?tE ?fE ?o => (eapply T_Const_add1)
-        | |- Typing ?E iszero' ?t ?tE ?fE ?o => (eapply T_Const_iszero)
-        | |- Typing ?E (expNum ?n) ?t ?tE ?fE ?o => (eapply T_Num)
-        | |- Typing ?E expT ?t ?tE ?fE ?o => (eapply T_True)
-        | |- Typing ?E expF ?t ?tE ?fE ?o => (eapply T_False)
-        | |- Typing ?E (expVar ?x) ?t ?tE ?fE ?o => (eapply T_Var)
-        | |- Typing ?E (expλ ?x ?t1 ?e) ?t' ?tE' ?fE' ?o' => (eapply T_Abs)
-        | |- Typing ?E (expApp ?e1 ?e2) ?t ?tE ?fE ?o => (eapply T_App)
-        | |- Typing ?E (expIf ?e1 ?e2 ?e3) ?t ?tE ?fE ?o => (eapply T_If)
-      end)).
-
-(* TODO 1: eautoT can try and match each directly, and if those fail
-         and it is really *some* typing goal, it can automatically
-         apply T_Subsume! This may or may not be a good idea... we'll
-         see i.e. *if* it is a Typing judgement, then try these
-         propermatches, and if those fail, try T_Subsume (or
-         something) 
-
-
-  TODO 2: Ltacs for the other relations *)
-
-Ltac eautoP :=
-  (try (repeat ((eapply P_Refl) || (eapply P_Empty)
-                  || (match goal with
-                          | |- Proves (envFalse ?E1) ?E2 => 
-                            (eapply P_False)
-                          | |- Proves ?E1 (envFact ?b ?t ?o ?E2) => 
-                            (eapply P_Fact_rhs)
-                          | |- Proves ?E1 (envFact ?b ?t ?o ?E2) => 
-                            (eapply P_Fact_rhs)
-                          | |- Proves ?E (envOr ?E1 ?E2) => 
-                            first [ (eapply P_Or_rhs_l) | (eapply P_Or_rhs_r)]
-                        end)
-                  || (match goal with
-                      | |- Proves (envOr ?E1 ?E2) ?E3 => 
-                        (eapply P_Or_lhs)
-                      | |- Proves (envFact ?b ?t ?o ?E1) ?E2 => 
-                        (eapply P_Fact_lhs)
-                     end)))).
-
-Ltac eautoPT :=
-  (try (repeat 
-         (match goal with
-          | ProvesTyping (tls_atom (Some tl)) true t o => eauto (* in progress *)
-          end)))
-
-Ltac crushTR :=
-repeat (try (eautoUE || eautoULS || eautoT || eautoP || eauto)).
 
 (*
 - Add if eqdec's to crushTR
@@ -1044,30 +1129,17 @@ repeat (try (eautoUE || eautoULS || eautoT || eautoP || eauto)).
 - add to outer match statement checks for simplifications (eqdecs, simpls of env_apps, etc)
  *)
 
-
 Lemma PT_empty_any : forall o,
 ProvesTyping (tls_atom emptylookup) true tTop o.
-Proof.
-  intros o.
-  eapply PT_Atom. eauto. eauto.
+Proof with crushTR.
+  intros o...
 Qed.  
 Hint Resolve PT_empty_any.
 
-Lemma neq_id_neq : forall (T:Type) x y (P Q:T),
-x <> y ->
-((if (id_eqdec x y) then P else Q) = Q).
+Theorem rescrap :
+Restricted tTop tNum tNum.
 Proof.
-  intros.
-  destruct (id_eqdec x y); crush.
-Qed.
 
-Lemma neq_obj_neq : forall (T:Type) x y (P Q:T),
-x <> y ->
-((if (obj_eqdec x y) then P else Q) = Q).
-Proof.
-  intros.
-  destruct (obj_eqdec x y); crush.
-Qed.
 
 (* Typing If statement where the if predicate/test passes
    it's conclusion to the then branch *)
@@ -1077,9 +1149,8 @@ Example example1:
                         (expApp add1' (expVar x)) 
                         (expNum 0))
                  tNum.
-Proof with crushTR. 
-  intros x.
-  eapply simpletype... simpl.  crushTR.
+Proof with crushTR.
+  intros x; eapply simpletype...
 Grab Existential Variables.
   crush. crush.
 Qed.
@@ -1095,21 +1166,11 @@ Example example2:
       (tUnion tBool tNum)
       (tBool).
 Proof with crushTR.
-  intros x.
-  eapply functiontype...
+  intros x; eapply functiontype... 
+  eapply T_Subsume...
 Grab Existential Variables.
   crush. crush.
 Qed.
-(* TODO: Applications of P_Fact... 
-   often lead to things like:
-
- UpdatedEnv
-     (envFact true (tUnion tBool tNum) (varx)
-        (envFact false tBool (varx) envEmpty)) (tls_atom None)
-
-Which is stupid, I should fix this if possible.
-
- *)
 
 
 (* Propositions from let-assignment are present in the let-body *)
@@ -1123,37 +1184,10 @@ Example example3:
                      (expNum 0)))
       tNum.
 Proof with crushTR.
-  intros x y Hneq.
-  eapply simpletype.
-  eapply (T_Let envEmpty 
-                (expApp isnum' (expVar y)) 
-                tBool 
-                (envFact true tNum (var y) envEmpty) 
-                (envFact false tNum (var y) envEmpty))...
-  eautoT... eapply (T_If tBool tNum). eautoT... eautoP... crushTR. crushTR. eautoUE...
-  eautoULS... eapply (UL_Some true tFalse tTop [] [] x)... eautoULS... 
-  eapply UL_Some... eautoULS... eapply (UL_Some true tFalse tTop [] [] x).
-  destruct (obj_eqdec (var y) (var x))... crush. crush.
-  eapply (UL_Some true tFalse tFalse [] [] x)... eautoULS.
-  eapply (UL_Some true tFalse tTop [] [] x)... eautoULS.
-  eapply (UL_Some true tNum tTop [] [] y)... eautoULS.
-  eapply (UL_Some true tNum tNum [] [] y)... 
-  eapply (UL_Some true tNum tTop [] [] y).
-  destruct (obj_eqdec (var x) (var y))... crush.
-  crush. eautoULS.
-  eapply (UL_Some true tBool tTop [] [] x).
-  destruct (obj_eqdec (vary) (varx))...
-  eapply UT_T... crush. 
-  eapply (UL_Some true tBool tFalse [] [] x). 
-  destruct (obj_eqdec (var y) (var x))... crush.
-  crush. eapply (UL_Some true tBool tFalse [] [] x)... 
-  eapply (UL_Some true tBool tFalse [] [] x)...
-  eapply PT_False_Cons. eapply PT_False_Cons. eapply PT_False_Cons.
-  eapply PT_Atom... eautoT... eapply P_Fact_rhs...
-  eautoUE. eautoULS...
-
+  intros x y Hneq; eapply simpletype...
+  eapply T_Subsume...
 Grab Existential Variables.
-  eauto. eauto.
+crush.
 Qed.
 
 (* Using or predicate to identify if x is of type (U Num Bool),
@@ -1162,15 +1196,58 @@ Qed.
  (Note also: the Union order is flipped, so it must use subtyping 
   to typecheck. )
  *)
+
+Definition f' (x:id) := (expλ x (tUnion tBool tNum) 
+            (expIf (expApp isbool' (expVar x)) 
+                   expF 
+                   (expApp iszero' (expVar x)))).
+
+Example example4prep:
+  forall x,
+    SimpleTypeOf
+      (expIf (expApp isnum' (expVar x)) 
+             expT 
+             (expApp isbool' (expVar x)))
+      tBool.
+Proof with crushTR.
+  intros x; eapply simpletype...
+  eapply T_Subsume...
+Grab Existential Variables.
+crush. crush.
+Qed.
+
 Example example4:
-  forall f x,
-    FunctionTypeOf (expVar f) (tUnion tNum tBool) (tBool) ->
+  forall x,
   SimpleTypeOf
-  (expIf (or' (expApp isnum' (expVar x)) (expApp isbool' (expVar x)))
-         (expApp (expVar f) (expVar x))
+  (expIf (expIf (expApp isnum' (expVar x)) expT (expApp isbool' (expVar x)))
+         (expApp (f' x) (expVar x))
          expF)
   tBool.
-Proof. Admitted. (* TODO! *)
+Proof with crushTR.
+  intros x.
+  eapply simpletype.
+  eapply T_If.
+  eapply T_If. (* BOOKMARK *)
+  crushTR.
+  crushTR.
+  crushTR.
+  crushTR.
+  crushTR.
+  crushTR.
+  crushTR.
+  eapply T_App.
+  tryT.
+  eapply T_Const_isbool.
+  tryT.
+  tryT.
+  crushTR.
+
+
+  intros x; eapply simpletype...
+  eapply T_Subsume...
+Grab Existential Variables.
+crush.
+Qed.
 
 (* usage of an and (nested ifs) to illustrate the conjunction of
    the predicates from the and being true *)
